progress:

Spacetalk/Compiler.lean
@@ -22,8 +22,8 @@ def Step.Prim.toSDFOpt : Step.Prim → SimpleDataflow.Ty
 structure SDFOneOutput (p : Step.Prim) where
   g : SimpleDataflow.DataflowMachine
   fifo : OutputFIFO g.outputs g.nodes
-  idx : Member (FIFO.output fifo) g.fifos
-  h_ty : fifo.t = p.toSDF
+  one_output : g.fifos.filter FIFO.isOutput = [.output fifo]
+  ty_eq : fifo.t = p.toSDF
 
 @[reducible]
 def Step.Ty.toSDF (sty : Step.Ty) :=
@@ -36,20 +36,20 @@ def binOpConstRightGraph {α β γ : Step.Prim} (op : SimpleDataflow.BinaryOp α
   let outputs := [γ.toSDF]
   let constNode := ⟨[], [β.toSDF], [], []ₕ, .const c⟩
   let opNode := ⟨[α.toSDF, β.toSDF], [γ.toSDF], [], []ₕ, .binaryOp op⟩
-  let nodes : SDFNodeList 2 := .cons constNode (.cons opNode .nil)
-  have h_eq : (nodes.get 1).outputs = [γ.toSDF] := by aesop
-  let outFifo : OutputFIFO outputs nodes := ⟨γ.toSDF, 1, h_eq ▸ .head, .head⟩
+  let nodes : SDFNodeList 2 := .cons opNode (.cons constNode .nil)
+  have h_eq : (nodes.get 0).outputs = [γ.toSDF] := by aesop
+  let outFifo : OutputFIFO outputs nodes := ⟨γ.toSDF, 0, h_eq ▸ .head, .head⟩
   let fifo := .output outFifo
   let fifos := [
-    .input ⟨α.toSDF, .head, 1, .head⟩,
-    .advancing ⟨β.toSDF, 0, 1, .head, .tail .head, _⟩,
+    .input ⟨α.toSDF, .head, 0, .head⟩,
+    .advancing ⟨β.toSDF, 1, 0, .head, .tail .head, _⟩,
     fifo
   ]
   let g : SimpleDataflow.DataflowMachine := ⟨inputs, outputs, 2, nodes, fifos⟩
   ⟨
     g,
     outFifo,
-    .tail (.tail .head),
+    by simp [fifos],
     by aesop
   ⟩
 
@@ -70,22 +70,9 @@ def binaryOpGraph {α β γ : Step.Prim} (op : SimpleDataflow.BinaryOp α.toSDF 
   ⟨
     g,
     (_ : outputs = g.outputs) ▸ outFifo,
-    .tail (.tail .head),
+    by simp [fifos],
     by aesop
   ⟩
-
-def isOutputFifo {numNodes : Nat} {inputs outputs : List SimpleDataflow.Ty} {nodes : SDFNodeList numNodes}
-  (outFifo : OutputFIFO outputs nodes) (fifo : FIFO inputs outputs nodes) : Bool :=
-  match fifo with
-    | .output f =>
-      if h_t : f.t = outFifo.t then
-        if h_p : f.producer = outFifo.producer then
-          and (f.producerPort == (h_t ▸ h_p ▸ outFifo.producerPort)) (f.consumer == (h_t ▸ outFifo.consumer))
-        else
-          false
-      else
-        false
-    | _ => false
 
 def Step.UnaryOp.compile : Step.UnaryOp α β → SDFOneOutput β
   | .addConst c => binOpConstRightGraph .add c
@@ -95,36 +82,100 @@ def Step.BinaryOp.compile : Step.BinaryOp α β γ → SimpleDataflow.Ops [α.to
   | .add => .binaryOp .add
   | .mul => .binaryOp .mul
 
+class IndexConverter {α : Type u} {n m : Nat} (xs : Vector α n) (ys : Vector α m) :=
+  conv : Fin n → Fin m
+  conv_congr : ∀ {i}, xs.get i = ys.get (conv i)
+  conv_lt : ∀ ⦃i j⦄, i < j → conv i < conv j
+
+def consConverter : IndexConverter xs (x ::ᵥ xs.append ys) :=
+  let conv : Fin xs.length → Fin (x ::ᵥ xs.append ys).length := λ i ↦ ⟨i.val + 1, by have := i.isLt; linarith⟩
+  let conv_congr : ∀ {i}, xs.get i = (x ::ᵥ xs.append ys).get (conv i) := by
+    intro i
+    rw [←(x ::ᵥ xs.append ys).get_tail ⟨i, Nat.lt_add_right _ i.isLt⟩]
+    exact Vector.get_append.symm
+  let conv_lt : ∀ ⦃i j⦄, i < j → conv i < conv j := by simp [conv]
+  ⟨conv, conv_congr, conv_lt⟩
+
+theorem consConverter_gt_zero : ∀ {i}, 0 < (@consConverter α n xs x m ys).conv i := by
+  intro i
+  simp [consConverter]
+  apply Fin.mk_lt_mk.mpr
+  rw [Nat.zero_mod]
+  simp
+
+def convertFifos {inputs outputs : List SimpleDataflow.Ty} {numNodes : Nat} {nodes : SDFNodeList numNodes}
+  (a : SDFOneOutput α) (newConsumer : Fin numNodes) (newConsumerPort : Member α.toSDF (nodes.get newConsumer).inputs)
+  (idxConv : IndexConverter a.g.nodes nodes)
+  (h_consumer_lt : ∀ {i}, newConsumer < idxConv.conv i)
+  (memConv : {t : SimpleDataflow.Ty} → Member t a.g.inputs → Member t inputs)
+  : List (FIFO inputs outputs nodes) :=
+  a.g.fifos.attach.map (
+    λ ⟨fifo, h_mem⟩ ↦ match fifo with
+      | .input f =>
+        let newConsumer := idxConv.conv f.consumer
+        let fifo : InputFIFO inputs nodes := {
+          t := f.t,
+          producer := memConv f.producer,
+          consumer := newConsumer,
+          consumerPort := idxConv.conv_congr ▸ f.consumerPort
+        }
+        .input fifo
+      | .output f =>
+        let newProducer := idxConv.conv f.producer
+        have h_ty_eq : f.t = α.toSDF := by
+          have : FIFO.output f = .output a.fifo := by
+            apply List.mem_singleton.mp
+            rw [←a.one_output]
+            apply List.mem_filter.mpr (And.intro h_mem (by rfl))
+          simp [FIFO.output.inj] at this
+          rw [this]
+          apply a.ty_eq
+        let fifo : AdvancingFIFO nodes := {
+          t := f.t,
+          producer := newProducer,
+          consumer := newConsumer,
+          producerPort := idxConv.conv_congr ▸ f.producerPort,
+          consumerPort := h_ty_eq ▸ newConsumerPort,
+          adv := h_consumer_lt,
+        }
+        .advancing fifo
+      | .advancing f =>
+        let newProducer := idxConv.conv f.producer
+        let newConsumer := idxConv.conv f.consumer
+        have adv : newProducer.val > newConsumer.val := by
+          simp [newProducer, newConsumer]
+          apply idxConv.conv_lt
+          exact f.adv
+        let fifo : AdvancingFIFO nodes := {
+          t := f.t,
+          producer := newProducer,
+          consumer := newConsumer,
+          producerPort := idxConv.conv_congr ▸ f.producerPort,
+          consumerPort := idxConv.conv_congr ▸ f.consumerPort,
+          adv := adv
+        }
+        .advancing fifo
+      | .initialized f =>
+        let newProducer := idxConv.conv f.producer
+        let newConsumer := idxConv.conv f.consumer
+        let fifo : InitializedFIFO nodes := {
+          t := f.t,
+          initialValue := f.initialValue,
+          producer := newProducer,
+          consumer := newConsumer,
+          producerPort := idxConv.conv_congr ▸ f.producerPort,
+          consumerPort := idxConv.conv_congr ▸ f.consumerPort,
+        }
+        .initialized fifo
+  )
+
 def mergeGraphs (a : SDFOneOutput α) (b : SDFOneOutput β) (op : Step.BinaryOp α β γ) : SDFOneOutput γ :=
   let inputs := a.g.inputs ++ b.g.inputs
   let outputs := [γ.toSDF]
   let newNode : SDFNode := ⟨[α.toSDF, β.toSDF], [γ.toSDF], [], []ₕ, op.compile⟩
   let nodes := newNode ::ᵥ (a.g.nodes.append b.g.nodes)
-  let aFifos := a.g.fifos.filter (isOutputFifo a.fifo)
-  let bFifos := b.g.fifos.filter (isOutputFifo b.fifo)
-  let aFifosUpdated : List (FIFO inputs outputs nodes) :=
-    aFifos.map (
-      λ fifo ↦ match fifo with
-        | .input f =>
-          let newConsumer : Fin nodes.length := ⟨f.consumer + 1, by
-            have := f.consumer.isLt
-            linarith
-          ⟩
-          have h_eq : nodes.get newConsumer = a.g.nodes.get f.consumer := by
-            let consumerIdxApp : Fin (a.g.numNodes + b.g.numNodes) := ⟨f.consumer, by apply Nat.lt_add_right; exact f.consumer.isLt⟩
-            rw [←nodes.get_tail consumerIdxApp]
-            simp [nodes]
-            apply Vector.get_append
-          let fifo : InputFIFO inputs nodes := {
-            producer := f.producer.append,
-            consumer := newConsumer,
-            consumerPort := h_eq ▸ f.consumerPort
-          }
-          .input fifo
-        | .output f => sorry
-        | .advancing f => sorry
-        | .initialized f => sorry
-    )
+
+  let aFifosUpdated : List (FIFO inputs outputs nodes) := convertFifos a 0 .head consConverter consConverter_gt_zero .append
   sorry
 
 def Step.Prog.compile {sty : Step.Ty} : Step.Prog sty → sty.toSDF
@@ -136,7 +187,6 @@ def Step.Prog.compile {sty : Step.Ty} : Step.Prog sty → sty.toSDF
   | Step.Prog.map op as => sorry
   | @Step.Prog.reduce α β op len init bs => sorry
   decreasing_by (all_goals sorry)
-
 
 
 -- def c : SimpleDataflow.Pipeline [] [SimpleDataflow.BoolTy] :=
